LeanStuff/Main.lean
@@ -1,5 +1,6 @@
 import LeanStuff
 import Lecture13
+import Lecture19
 
 def main : IO Unit :=
   IO.println s!"Hello, {hello}!"
